Subtyping relation

src/Coq/Syntax.v
@@ -2,45 +2,67 @@ Require Import List.
 
 Notation Id := nat.
 Notation "'[' X ']'" := (list X) (at level 40).
-(* We will use Notation to make automation easier*)
+(* We will use Notation to make automation easier
+ * This will be the notation to be similar with haskell *)
 
-Inductive ClassName : Type :=
+Inductive ClassName :=
   | ClassObject : ClassName
   | ClassId : Id -> ClassName.
  
-Inductive Var : Type :=
+Inductive Var :=
   | This : Var
   | VarId: Id -> Var.
 
-Inductive Argument : Type :=
+Inductive Argument :=
   | Arg : Id -> Argument.
 
-Inductive Assignment : Type :=
+Inductive Assignment :=
   | Assgnmt : Id -> Id -> Assignment.
 
-Inductive FormalArg : Type :=
+Inductive FormalArg :=
   | FArg : ClassName -> Id -> FormalArg.
 
-Inductive Constructor : Type :=
+Inductive Constructor :=
   | KDecl : Id -> [FormalArg] -> [Argument] -> [Assignment] -> Constructor.
 
-Inductive FieldDecl : Type :=
+Inductive FieldDecl :=
   | FDecl : ClassName -> Id -> FieldDecl.
 
-Inductive Exp : Type :=
+Inductive Exp :=
   | ExpVar : Var -> Exp
   | ExpFieldAccess : Exp -> Id -> Exp
   | ExpMethodInvoc: Exp -> Id -> [Exp] -> Exp
   | ExpCast : ClassName -> Exp -> Exp
   | ExpNew : Id -> [Exp] -> Exp.
 
-Inductive MethodDecl : Type :=
+Inductive MethodDecl :=
   | MDecl : ClassName -> Id -> [FormalArg] -> Id -> MethodDecl.
 
-Inductive ClassDecl : Type :=
+Inductive ClassDecl :=
   | CDecl: Id -> ClassName -> [FieldDecl] -> Constructor -> [MethodDecl] -> ClassDecl.
 
-Inductive Program : Type :=
+Inductive Program :=
   | CProgram : [ClassDecl] -> Exp -> Program.
 
+Parameter CT: [ClassDecl].
+(*We will assume a global CT to make our definitions easier
+ *To instance the CT use Hypothesis x: CT = ... *)
+
+Definition extends (C D : ClassName) : Prop :=
+  match C with
+  | ClassObject => False
+  | ClassId cname =>
+    exists fdecls kons mdecl, List.In (CDecl cname D fdecls kons mdecl) CT
+  end.
+
+
+Reserved Notation "C '<:' D " (at level 40).
+
+Inductive Subtype : ClassName -> ClassName -> Set :=
+  | S_Refl: forall C:ClassName, C <: C
+  | S_Trans: forall (C D E: ClassName), 
+    C <: D -> D <: E -> C <: E
+  | S_Decl: forall C D, 
+    extends C D -> C <: D
+where "C '<:' D" := (Subtype C D).
 
