src/Coq/Examples.v
@@ -1,0 +1,12 @@
+Require Import Syntax.
+Require Import List.
+Hypothesis ct_fix : CT = (CDecl 1 (ClassObject) nil (KDecl 1 nil nil nil) nil) :: nil .
+
+Lemma ex: (ClassId 1 <: ClassObject).
+  apply S_Decl.
+  unfold extends.
+  rewrite ct_fix.
+  simpl.
+  eauto.
+Qed.
+
